More debugging of [Equations], now able to discharge even the heavily dependent [noConfusion] definitions in "A Few Constructions on Constructors". Now the guardness check is blocking.
git-svn-id: svn+ssh://scm.gforge.inria.fr/svn/coq/trunk@11374 85f007b7-540e-0410-9357-904b9bb8a0f7

proofs/logic.ml
@@ -57,6 +57,8 @@ let rec catchable_exception = function
 		   |NoOccurrenceFound _|CannotUnifyBindingType _|NotClean _
 		   |CannotFindWellTypedAbstraction _
 		   |UnsolvableImplicit _)) -> true
+  | Typeclasses_errors.TypeClassError 
+      (_, Typeclasses_errors.UnsatisfiableConstraints _) -> true
   | _ -> false
 
 (* Tells if the refiner should check that the submitted rules do not
